---

# title: 5.5. Scheduling: Minimizing Total Time in the System 
tags: alg
category: alg
picture_frame: shadow
use_math: true
---
# 5.5. Scheduling: Minimizing Total Time in the System 

- Problem
  - Consider a system in which a server is about to serve n clients. Let $T = {t_1, t_2, ..., t_n}$ be a set of positive numbers, where $ti$ is the estimated **time-to-completion** for the ith client. What is the optimal order of service where **the $total (wait+service)$ time in the system is minimized?**
  - Hair stylist with waiting clients, pending operations on a shared hard disk, etc.
- Example
  - $T = {t_1, t_2, t_3} = {5, 10, 4}$
    | Schedule  | Total Time in the System          |
    | --------- | --------------------------------- |
    | $[1, 2, 3]$ | $5 + (5 + 10) + (5 + 10 + 4) = 39$  |
    | $[1, 3, 2]$ | $33$                                |
    | $[2, 1, 3]$ | $10 + (10 + 5) + (10 + 5 + 4) = 44$ |
    | $[2, 3, 1]$ | $43$                                | 
    | $[3, 1, 2]$ | $☞ 4 + (4 + 5) + (4 + 5 + 10) = 32$ |
    | $[3, 2, 1]$ | $37$                                |
- A naïve approach
  - Enumerate all possible schedules of service, and select the optimal one.
    → $O(n!)$
- A greedy approach
  - Algorithm 
    - Sort $T$ in nondecreasing order to get the optimal schedule. - → $O(n \log n)$
  - Correctness : 귀류법 (Proof by contradiction)
    - Does the greedy approach always find a schedule that minimizes the total time in the system?
    - Let $S = [s_1, s_2, ..., s_n]$ be an optimal schedule, and $C(S)$ be the total time for $S$. 
    - $C(S) = s_1 + (s_1 +s_2) + (s_1 + s_2 + s_3) + ... + (s_1 + s_2 + ... + s_n) \\ = n \cdot s_1 + (n-1) \cdot s_2 + ... + 2 \cdot s_{n-1} + 1 \cdot s_n \\ = \Sigma_{i=1}^{n}{(n+1-i)\cdot s_i} \\ = (n+1) \Sigma_{i=1}^{n}{s_i}-\Sigma_{i=1}^{n}{i \cdot s_i}$ 
    - If they are not scheduled in nondecreasing order, then, for at least one $i(1≤i≤n-1)$,$s_i >s_{i+1}$.
    - Now consider the schedule $S’ = [s_1, s_2, ..., s_{i+1}, si, ..., sn]$ that is obtained by interchanging $s_i$ and $s_{i+1}$.
    - Then,$C(s) - C(s') \\ = (i \cdot s_{i+1} + (i+1) \cdot s_i) - (i \cdot s_i + (i+1) \cdot s_{i+1}) \\ = s_i - s_{i+1} >0$. 
    - Therefore, ...
